

OVSP definitions

Protocol specification

$$\begin{aligned} \text{RoleTerm} ::= & \text{Var} \mid \text{Fresh} \mid \text{Role} \mid \text{Func}(\text{RoleTerm}^*) \\ & \mid (\text{RoleTerm}, \text{RoleTerm}) \mid \{\!\{ \text{RoleTerm} \}\!\}_{\text{RoleTerm}} \\ & \mid \text{sk}(\text{RoleTerm}) \mid \text{pk}(\text{RoleTerm}) \mid k(\text{RoleTerm}, \text{RoleTerm}) \end{aligned}$$

$$\begin{aligned} \text{RoleEvent}_R ::= & \text{send}_{\text{Label}}(R, \text{Role}, \text{RoleTerm}) \\ & \mid \text{recv}_{\text{Label}}(\text{Role}, R, \text{RoleTerm}) \\ & \mid \text{claim}_{\text{Label}}(R, \text{Claim}, [\text{RoleTerm}]) \end{aligned}$$

$$\text{RoleEvent} = \bigcup_{R \in \text{Role}} \text{RoleEvent}_R$$

$$P(R) = (KN_0(R), s) \in \mathcal{P}(\text{RoleTerm}) \times \text{RoleEvent}_R^*$$

$$\begin{aligned} \text{RoleSpec} = \{ & (kn, s) \mid kn \in \mathcal{P}(\text{RoleTerm}) \wedge \forall rt(rt \in kn \rightarrow \text{vars}(rt) = \emptyset) \\ & \wedge s \in \text{RoleEvent}^* \wedge \text{wellformed}(s) \} \end{aligned}$$

$$\text{Protocol} = \text{Role} \rightarrow \text{RoleSpec}$$

Deduction on terms

$M \vdash t$ means that t can be deduced knowing M

\vdash is the least relation with the following properties:

$$\begin{aligned} \text{if } & t \in M \quad \text{then } M \vdash t \\ \text{if } & M \vdash t_1 \text{ and } M \vdash t_2 \quad \text{then } M \vdash (t_1, t_2) \\ \text{if } & M \vdash (t_1, t_2) \quad \text{then } M \vdash t_1 \text{ and } M \vdash t_2 \\ \text{if } & M \vdash t \text{ and } M \vdash k \quad \text{then } M \vdash \{\!\{ t \}\!\}_k \\ \text{if } & M \vdash \{\!\{ t \}\!\}_k \text{ and } M \vdash k^{-1} \quad \text{then } M \vdash t \\ \text{if } & M \vdash t_1 \text{ and } \dots \text{ and } M \vdash t_n \quad \text{then } M \vdash f(t_1, \dots, t_n) \end{aligned}$$

Protocol execution

$$\begin{aligned} \text{RunTerm} ::= & \text{Var}^{\#RID} \mid \text{Fresh}^{\#RID} \mid \text{Role}^{\#RID} \mid \text{Agent} \mid \text{Func}(\text{RunTerm}^*) \\ & \mid (\text{RunTerm}, \text{RunTerm}) \mid \{\!\{ \text{RunTerm} \}\!\}_{\text{RunTerm}} \\ & \mid \text{AdversaryFresh} \\ & \mid \text{sk}(\text{RunTerm}) \mid \text{pk}(\text{RunTerm}) \mid k(\text{RunTerm}, \text{RunTerm}) \end{aligned}$$

$$\text{Inst} = RID \times (\text{Role} \rightarrow \text{Agent}) \times (\text{Var} \rightarrow \text{RunTerm}) \quad \text{inst} = (\theta, \rho, \sigma) \in \text{Inst}$$

$$\text{Run} = \text{Inst} \times \text{RoleEvent}^*$$

Operational semantics

$$\text{State} = \mathcal{P}(\text{RunTerm}) \times \mathcal{P}(\text{Run})$$

$st = \langle\langle \text{AKN}, F \rangle\rangle \in \text{State}$ where

AKN is the adversary knowledge and $F \subseteq \text{Run}$ are the runs that has to be executed.

$$\text{RunEvent} = \text{Inst} \times (\text{RoleEvent} \cup \{\text{create}(R) \mid R \in \text{Role}\})$$

Labeled Transition System for Operational Semantics: $(\text{State}, \text{RunEvent}, \rightarrow, st_0(P))$

where $st_0(P) = \langle\langle \text{AKN}_0(P), \emptyset \rangle\rangle$ where $\text{AKN}_0(P)$ is the initial adversary knowledge.

Transition rules for $(\text{State}, \text{RunEvent}, \rightarrow, st_0(P))$:

- $[create_P] \frac{R \in dom(P) \quad ((\theta, \rho, \emptyset), s) \in runsof(P, R) \quad \theta \notin runsIDs(F)}{\langle\langle AKN, F \rangle\rangle \xrightarrow{((\theta, \rho, \emptyset), create(R))} \langle\langle AKN, F \cup \{((\theta, \rho, \emptyset), s)\}\rangle\rangle}$
- $[send] \frac{e = send_l(R_1, R_2, m) \quad (inst, [e] \cdot s) \in F}{\langle\langle AKN, F \rangle\rangle \xrightarrow{(inst, e)} \langle\langle AKN \cup \{inst(m)\}, F \setminus \{(inst, [e] \cdot s)\} \cup \{(inst, s)\}\rangle\rangle}$
 - $[send]$ is the only rule that **changes the adversary knowledge**
- $[recv] \frac{e = recv_l(R_1, R_2, pt) \quad AKN \vdash m \quad (inst, [e] \cdot s) \in F \quad Match(inst, pt, m, inst')}{\langle\langle AKN, F \rangle\rangle \xrightarrow{(inst', e)} \langle\langle AKN, F \setminus \{(inst, [e] \cdot s)\} \cup \{(inst', s)\}\rangle\rangle}$
- $[claim] \frac{e = claim_l(R, c, t) \quad (inst, [e] \cdot s) \in F}{\langle\langle AKN, F \rangle\rangle \xrightarrow{(inst, e)} \langle\langle AKN, F \setminus \{(inst, [e] \cdot s)\} \cup \{(inst, s)\}\rangle\rangle}$

The Needham-Schroeder protocol

$$\begin{array}{ll}
 NS(i) = & (\{i, r, ni, sk(i), pk(i), pk(r)\}, \\
 & [send_1(i, r, \{ \{ ni, i \} \}_{pk(r)}), \\
 & recv_2(r, i, \{ \{ ni, V \} \}_{pk(i)}), \\
 & send_3(i, r, \{ \{ V \} \}_{pk(r)}), \\
 & claim_4(i, synch)]) \\
 NS(r) = & (\{i, r, nr, sk(r), pk(r), pk(i)\}, \\
 & [recv_1(i, r, \{ \{ W, i \} \}_{pk(r)}), \\
 & send_2(r, i, \{ \{ W, nr \} \}_{pk(i)}), \\
 & recv_3(i, r, \{ \{ nr \} \}_{pk(r)}), \\
 & claim_5(r, synch)])
 \end{array}$$

$$AKN_0(NS) = AdversaryFresh \cup Agent \cup \{pk(A) \mid A \in Agent\} \cup \{sk(A) \mid A \in Agent_C\}$$